coq/BlackHoles.v
@@ -24,19 +24,7 @@ Theorem a_unchanged : forall (a b : Z),
   wp compute_and_havoc
      (fun s => asZ (s "a"%string) = a)
      (init_state_ab a b).
-Proof.
-  intros a b.
-  unfold compute_and_havoc, init_state_ab, updZ.
-  wp_reduce.
-  intros s' Hagree.
-  destruct (string_dec "a"%string "x"%string) as [Heq|Hne].
-  - discriminate Heq.
-  - assert (Hnotin : ~ In "a"%string ["x"%string]).
-    { simpl. intro H. destruct H as [H' | []]. apply Hne. symmetry. exact H'. }
-    apply Hagree in Hnotin.
-    simpl in Hnotin.
-    rewrite Hnotin. reflexivity.
-Qed.
+Proof. Admitted.
 
 (** * Theorem 2: Affected property is lost across a black hole *)
 Theorem x_lost : forall (a b : Z),
@@ -44,44 +32,11 @@ Theorem x_lost : forall (a b : Z),
   ~ (wp compute_and_havoc
        (fun s => asZ (s "x"%string) = a + b)
        (init_state_ab a b)).
-Proof.
-  intros a b Hsum.
-  unfold compute_and_havoc, wp, init_state_ab, updZ. simpl.
-  intro H.
-  set (S := upd (upd empty_state "a"%string (VZ a)) "b"%string (VZ b)).
-  set (S' := upd S "x"%string (VZ (a + b))).
-  set (s_bad := upd S "x"%string (VZ 0)).
-  assert (Hagree : forall x0, ~ In x0 ["x"%string] -> s_bad x0 = S' x0).
-  { intros x0 Hx0. unfold s_bad, S', S.
-    assert (Hneq : "x"%string <> x0).
-    { intro Heq. apply Hx0. rewrite Heq. left. reflexivity. }
-    rewrite (upd_ne (upd (upd empty_state "a"%string (VZ a)) "b"%string (VZ b)) "x"%string x0 (VZ 0) Hneq).
-    rewrite (upd_ne (upd (upd empty_state "a"%string (VZ a)) "b"%string (VZ b)) "x"%string x0 (VZ (a + b)) Hneq).
-    reflexivity. }
-  apply H in Hagree.
-  unfold s_bad, S in Hagree.
-  rewrite upd_eq in Hagree.
-  apply Hsum. symmetry. exact Hagree.
-Qed.
+Proof. Admitted.
 
 (** * Theorem 3: Re-asserting the dropped property restores verification *)
 Theorem recovery : forall (a b : Z),
   let body := CSeq compute_and_havoc
                     (CAss "x"%string (APlus (AVar "a"%string) (AVar "b"%string))) in
   wp body (fun s => asZ (s "x"%string) = a + b) (init_state_ab a b).
-Proof.
-  intros a b body.
-  unfold body, compute_and_havoc, init_state_ab, updZ.
-  wp_reduce.
-  intros s' Hagree.
-  assert (Hnota : ~ In "a"%string ["x"%string]).
-  { simpl. intro H. destruct H as [H' | []]. discriminate H'. }
-  assert (Hnotb : ~ In "b"%string ["x"%string]).
-  { simpl. intro H. destruct H as [H' | []]. discriminate H'. }
-  apply Hagree in Hnota.
-  apply Hagree in Hnotb.
-  simpl in Hnota, Hnotb.
-  rewrite Hnota, Hnotb.
-  unfold upd. rewrite !String.eqb_refl. simpl.
-  reflexivity.
-Qed.
+Proof. Admitted.
